Algorithm.lean
@@ -2,6 +2,7 @@ import Algorithm.Algebra.BigOperators.DFinsupp'
 import Algorithm.Data.Classes.AssocArray
 import Algorithm.Data.Classes.Bag
 import Algorithm.Data.Classes.Dict
+import Algorithm.Data.Classes.Erase
 import Algorithm.Data.Classes.GetElem
 import Algorithm.Data.Classes.IndexedMinHeap
 import Algorithm.Data.Classes.MinHeap
