Algorithm/Data/Classes/MultiBag.lean
@@ -19,7 +19,8 @@ export MultiBag.ReadOnly (count count_eq_count_toMultiset)
 class MultiBag (C : Type*) (α : outParam Type*) extends
     MultiBag.ReadOnly C α,
     EmptyCollection C, LawfulEmptyCollection C α,
-    Insert α C, ToMultiset.LawfulInsert C α
+    Insert α C, ToMultiset.LawfulInsert C α,
+    Erase C α, LawfulErase C α
 
 attribute [instance 100] MultiBag.ReadOnly.decidableMem
 
